CertifyingDatalog/Unification.lean
@@ -1,6 +1,6 @@
 import CertifyingDatalog.Datalog
 
-section matching
+section term_matching
 variable {τ: signature} [DecidableEq τ.constants][DecidableEq τ.vars]
 
 def extend (s: substitution τ) (v: τ.vars) (c: τ.constants) : substitution τ := fun x => if x = v then Option.some c else s x
@@ -23,7 +23,7 @@ by
   | none =>
     simp
 
-def match_term (t: term τ)(c: τ.constants) (s: substitution τ): Option (substitution τ) :=
+def matchTerm (t: term τ)(c: τ.constants) (s: substitution τ): Option (substitution τ) :=
   match t with
   | term.constant c' =>
     if c = c'
@@ -39,129 +39,405 @@ def match_term (t: term τ)(c: τ.constants) (s: substitution τ): Option (subst
     else
       extend s v c
 
-lemma matchTermIsSomeIffSolution (t: term τ) (c: τ.constants): Option.isSome (match_term t c (fun _ => Option.none)) ↔ ∃ (s: substitution τ), applySubstitutionTerm s t = c :=
-by
-  simp
-  constructor
-  intro h
-  use Option.get (match_term t c (fun _ => Option.none)) h
-  cases t with
-    | constant c' =>
-      unfold match_term
-      simp
-      by_cases p: c= c'
-      simp [p]
-      unfold applySubstitutionTerm
-      simp
-      exfalso
-      unfold match_term at h
-      simp [p] at h
-    | variableDL v =>
-      unfold match_term
-      simp
-      unfold extend
-      unfold applySubstitutionTerm
-      simp
-  by_contra h
-  simp at h
-  rcases h with ⟨s, none⟩
-  rcases s with ⟨s, s_prop⟩
-  cases t with
-  | constant c' =>
-    unfold match_term at none
-    simp at none
-    by_cases p: c' = c
-    simp [p] at none
-    unfold applySubstitutionTerm at s_prop
-    simp at s_prop
-    exact absurd s_prop p
-  | variableDL v =>
-    unfold match_term at none
-    simp at none
-
-lemma matchTermFindsMinimalSolution (t: term τ) (c: τ.constants) (s: substitution τ) (h: Option.isSome (match_term t c s)): applySubstitutionTerm (Option.get (match_term t c s) h) t = c ∧ s ⊆ (Option.get (match_term t c s) h) ∧ ∀ (s': substitution τ), (s ⊆ s' ∧ applySubstitutionTerm s' t = c) → (Option.get (match_term t c s) h) ⊆ s' :=
+lemma matchTermFindsSolution (t: term τ) (c: τ.constants) (s: substitution τ) (h: Option.isSome (matchTerm t c s)): applySubstitutionTerm (Option.get (matchTerm t c s) h) t = c ∧ s ⊆ (Option.get (matchTerm t c s) h) :=
 by
   cases t with
   | constant c' =>
     simp
-    unfold match_term at h
+    unfold matchTerm at h
     simp at h
     have c_c': c = c'
     by_contra h'
     simp [h'] at h
     constructor
-    unfold match_term
+    unfold matchTerm
     unfold applySubstitutionTerm
     simp [c_c']
-    constructor
-    unfold match_term
+    unfold matchTerm
     simp [c_c']
     apply substitution_subs_refl
-    intros s' s_s' _
-    unfold match_term
-    simp [c_c', s_s']
   | variableDL v =>
-    unfold match_term at h
+    unfold matchTerm at h
     by_cases p: Option.isSome (s v)
     have sv_c: Option.get (s v) p = c
     by_contra h'
     simp [p, h'] at h
-    have h': (Option.get (match_term (term.variableDL v) c s) h) = s
-    unfold match_term
+    have h': (Option.get (matchTerm (term.variableDL v) c s) h) = s
+    unfold matchTerm
     simp [p, sv_c]
     simp
     constructor
     rw [h']
     unfold applySubstitutionTerm
     simp [p, sv_c]
-    constructor
     rw [h']
     apply substitution_subs_refl
-    intro s' s_s' _
-    rw [h']
-    apply s_s'
-    have h': Option.get (match_term (term.variableDL v) c s) h = extend s v c
-    unfold match_term
+    have h': Option.get (matchTerm (term.variableDL v) c s) h = extend s v c
+    unfold matchTerm
     simp [p]
     rw [h']
     constructor
     unfold applySubstitutionTerm
     unfold extend
     simp
-    constructor
     apply s_subset_extend_s
     simp at p
     apply p
-    by_contra not_min
-    push_neg at not_min
-    rcases not_min with ⟨s', right⟩
-    rcases right with ⟨left, not_extend⟩
-    rcases left with ⟨s_s', apply_s'⟩
-    unfold_projs at not_extend
-    unfold substitution_subs at not_extend
-    push_neg at not_extend
-    unfold extend at not_extend
-    rcases not_extend with ⟨v', not_subs⟩
-    by_cases v'_v: v' = v
-    simp [v'_v] at not_subs
-    have s'v_c: s' v = some c
-    unfold applySubstitutionTerm at apply_s'
-    simp at apply_s'
-    by_cases p': Option.isSome (s' v)
-    simp [p'] at apply_s'
-    rw [Option.eq_some_iff_get_eq]
-    simp [apply_s']
-    apply p'
-    simp [p'] at apply_s'
-    simp [s'v_c] at not_subs
 
-    simp [v'_v] at not_subs
-    cases sv': s v' with
+lemma matchTermFindsMinimalSolution' (t: term τ) (c: τ.constants) (s: substitution τ) (h: Option.isSome (matchTerm t c s)): ∀ (s': substitution τ), (s ⊆ s' ∧ applySubstitutionTerm s' t = c) → (Option.get (matchTerm t c s) h) ⊆ s' :=
+by
+  cases t with
+  | constant c' =>
+    unfold matchTerm at h
+    simp at h
+    have c_c': c = c'
+    by_contra h'
+    simp [h'] at h
+    intros s' s'_prop
+    unfold matchTerm
+    simp [c_c', s'_prop]
+  | variableDL v =>
+    intros s' s_s'
+    rcases s_s' with ⟨s_s', apply_s'⟩
+    unfold matchTerm at h
+    simp at h
+    unfold matchTerm
+    by_cases p: Option.isSome (s v) = true
+    have h': Option.get (s v) p = c
+    by_contra p'
+    simp [p, p'] at h
+    simp [p, h']
+    simp [s_s']
+    simp [p]
+    by_contra h'
+    unfold_projs at h'
+    unfold substitution_subs at h'
+    unfold extend at h'
+    simp at h'
+    rcases h' with ⟨x, x_prop⟩
+    by_cases x_v: x = v
+    simp [x_v] at x_prop
+    cases sv: s' v with
     | some c' =>
-      simp [sv'] at not_subs
-      have s'_v': s' v' = some c'
-      apply substitution_subs_get s s' s_s' _ _ sv'
-      simp[s'_v'] at not_subs
+      simp [sv] at x_prop
+      unfold applySubstitutionTerm at apply_s'
+      have p': Option.isSome (s' v) = true
+      rw [sv]
+      simp
+      simp [p'] at apply_s'
+      rw [option_get_iff_eq_some] at apply_s'
+      simp [apply_s'] at sv
+      exact absurd sv x_prop
     | none =>
-      simp [sv'] at not_subs
-end matching
+      unfold applySubstitutionTerm at apply_s'
+      simp [sv] at apply_s'
+    simp [x_v] at x_prop
+    cases q:s x with
+    | some c =>
+      simp [q] at x_prop
+      have s'x: s' x = some c
+      apply substitution_subs_get s s' s_s' _ _ q
+      simp [s'x] at x_prop
+    | none =>
+      simp [q] at x_prop
+
+lemma matchTermNoneImpNoSolution (t: term τ) (c: τ.constants) (s: substitution τ) (h: Option.isNone (matchTerm t c s)): ¬ (∃(s': substitution τ), s ⊆ s' ∧ applySubstitutionTerm s' t = c) :=
+by
+  push_neg
+  unfold matchTerm at h
+  cases t with
+  | constant c' =>
+    simp at h
+    have c_c': ¬ c' = c
+    by_contra h'
+    simp [h'] at h
+    intros s' _
+    unfold applySubstitutionTerm
+    simp [c_c']
+  | variableDL v =>
+    simp at h
+    have h': Option.isSome (s v) = true
+    by_contra p
+    simp [p] at h
+    simp [h'] at h
+    have p: ¬ Option.get (s v) h' = c
+    by_contra q
+    simp [q] at h
+    intros s' s_s'
+    unfold applySubstitutionTerm
+    unfold_projs at s_s'
+    unfold substitution_subs at s_s'
+    specialize s_s' v
+    simp
+    rw [Option.isSome_iff_exists] at h'
+    rcases h' with ⟨c', sv_c'⟩
+    simp [sv_c'] at s_s'
+    by_cases q: Option.isSome (s' v) = true
+    simp [q]
+    rw [Option.isSome_iff_exists] at q
+    rcases q with ⟨b,s'v_b⟩
+    simp [s'v_b] at *
+    rw [← s_s']
+    simp [sv_c'] at h
+    by_contra q
+    simp [q] at h
+    simp [q]
+
+lemma matchTermIsSomeIffSolution (t: term τ) (c: τ.constants): Option.isSome (matchTerm t c emptySubstitution) ↔ ∃ (s: substitution τ), applySubstitutionTerm s t = c :=
+by
+  constructor
+  intro h
+  use Option.get (matchTerm t c emptySubstitution) h
+  simp [matchTermFindsSolution]
+
+  by_contra h
+  push_neg at h
+  rcases h with ⟨left, right⟩
+  simp at right
+  have h': ¬ ∃ s, emptySubstitution ⊆ s ∧ applySubstitutionTerm s t = term.constant c
+  apply matchTermNoneImpNoSolution (h:= right)
+  push_neg at h'
+  rcases left with ⟨s, s_prop⟩
+  specialize h' s
+  have p: emptySubstitution ⊆ s
+  apply emptySubstitutionIsMinimal
+  specialize h' p
+  exact absurd s_prop h'
+
+
+end term_matching
+
+section atom_matching
+variable {τ: signature} [DecidableEq τ.constants][DecidableEq τ.vars] [DecidableEq τ.relationSymbols]
+
+def matchTermList (s: substitution τ) (l1: List (term τ)) (l2: List (τ.constants)): Option (substitution τ) :=
+  match l1 with
+  | List.nil => some s
+  | List.cons hd tl =>
+    match l2 with
+    | List.nil => none
+    | List.cons hd' tl' =>
+      let s' := matchTerm hd hd' s
+      if p: Option.isSome s'
+      then matchTermList (Option.get s' p) tl tl'
+      else none
+
+lemma matchTermListFindsSolution (s: substitution τ) (l1: List (term τ)) (l2: List (τ.constants)) (len: l1.length = l2.length) (h: Option.isSome (matchTermList s l1 l2)): List.map (applySubstitutionTerm (Option.get (matchTermList s l1 l2) h ) ) l1 = List.map term.constant l2 ∧ s ⊆ (Option.get (matchTermList s l1 l2) h ) :=
+by
+  induction l1 generalizing l2 s with
+  | nil =>
+    cases l2 with
+    | nil =>
+      constructor
+      simp
+      unfold matchTermList
+      simp
+      apply substitution_subs_refl
+    | cons hd tl =>
+      simp at len
+  | cons hd tl ih =>
+    cases l2 with
+    | nil =>
+      simp at len
+    | cons hd' tl' =>
+      simp at len
+      unfold matchTermList at h
+      simp at h
+      have p : Option.isSome (matchTerm hd hd' s) = true
+      by_contra p'
+      simp [p'] at h
+      simp [p] at h
+      constructor
+      simp
+      constructor
+      unfold matchTermList
+      simp [p]
+      apply subs_ext_groundTerm (s1:= Option.get (matchTerm hd hd' s) p)
+      specialize ih (Option.get (matchTerm hd hd' s) p) tl' len h
+      simp [ih]
+      simp [matchTermFindsSolution]
+
+      unfold matchTermList
+      simp [p, h]
+      specialize ih (Option.get (matchTerm hd hd' s) p) tl' len h
+      simp [ih]
+
+      unfold matchTermList
+      simp [p,h]
+      apply substitution_subs_trans (s2:= Option.get (matchTerm hd hd' s) p)
+      simp [matchTermFindsSolution]
+      specialize ih (Option.get (matchTerm hd hd' s) p) tl' len h
+      simp [ih]
+
+lemma matchTermListFindsMinimalSolution (s: substitution τ) (l1: List (term τ)) (l2: List (τ.constants)) (len: l1.length = l2.length) (h: Option.isSome (matchTermList s l1 l2)):∀ (s': substitution τ), List.map (applySubstitutionTerm s') l1 = List.map term.constant l2 ∧ s ⊆ s' → (Option.get (matchTermList s l1 l2) h ) ⊆ s' :=
+by
+  induction l1 generalizing l2 s with
+  | nil =>
+    intros s' s'_prop
+    unfold matchTermList
+    simp [s'_prop]
+  | cons hd tl ih=>
+    cases l2 with
+    | nil =>
+      simp at len
+    | cons hd' tl' =>
+      intros s' s'_prop
+      unfold matchTermList
+      unfold matchTermList at h
+      have p : Option.isSome (matchTerm hd hd' s) = true
+      by_contra p'
+      simp [p'] at h
+      simp [p]
+      apply ih
+      simp at len
+      apply len
+      constructor
+      simp at s'_prop
+      simp [s'_prop]
+      apply matchTermFindsMinimalSolution'
+      constructor
+      simp [s'_prop]
+      simp at s'_prop
+      simp [s'_prop]
+
+lemma matchTermListNoneImplNoSolution (s: substitution τ) (l1: List (term τ)) (l2: List (τ.constants)) (len: l1.length = l2.length) (h: Option.isNone (matchTermList s l1 l2)): ¬ ∃ (s': substitution τ), s ⊆ s' ∧ List.map (applySubstitutionTerm s') l1 = List.map term.constant l2 :=
+by
+  push_neg
+  intros s' s_s'
+  induction l1 generalizing l2 s with
+  | nil =>
+    cases l2 with
+    | nil =>
+      unfold matchTermList at h
+      simp at h
+    | cons hd tl =>
+      simp at len
+  | cons hd tl ih =>
+    cases l2 with
+    | nil =>
+      simp at len
+    | cons hd' tl' =>
+      unfold matchTermList at h
+      simp at h
+      by_cases p : Option.isSome (matchTerm hd hd' s) = true
+      simp [p] at h
+      specialize ih (Option.get (matchTerm hd hd' s) p) tl'
+      simp
+      intro s'_hd
+      apply ih
+      simp at len
+      apply len
+      apply h
+      apply matchTermFindsMinimalSolution'
+      constructor
+      apply s_s'
+      simp [s'_hd]
+
+      simp at p
+      have h': ¬ ∃ (s1: substitution τ), s ⊆ s1 ∧ applySubstitutionTerm s1 hd = hd'
+      apply matchTermNoneImpNoSolution (h:= p)
+      push_neg at h'
+      specialize h' s' s_s'
+      simp [h']
+
+def matchAtom (s: substitution τ) (a: atom τ) (ga: groundAtom τ): Option (substitution τ) :=
+  if a.symbol = ga.symbol
+  then
+    if a.atom_terms.length = ga.atom_terms.length
+    then matchTermList s a.atom_terms ga.atom_terms
+    else none
+  else none
+
+lemma matchAtomFindsSolution (s: substitution τ) (a: atom τ) (ga: groundAtom τ) (h: Option.isSome (matchAtom s a ga)): applySubstitutionAtom (Option.get (matchAtom s a ga) h) a = ga ∧ s ⊆ (Option.get (matchAtom s a ga) h) :=
+by
+  unfold matchAtom at h
+  have symbol_eq: a.symbol = ga.symbol
+  by_contra p
+  simp [p] at h
+  have length_eq: a.atom_terms.length = ga.atom_terms.length
+  by_contra p
+  simp [symbol_eq, p] at h
+  simp [symbol_eq, length_eq] at h
+  unfold matchAtom
+  simp [symbol_eq, length_eq]
+  unfold applySubstitutionAtom
+  unfold groundAtom.toAtom
+  simp [ruleEquality]
+  rw [and_assoc]
+  constructor
+  apply symbol_eq
+  apply matchTermListFindsSolution (len:= length_eq)
+
+lemma matchAtomFindsMinimalSolution (s: substitution τ) (a: atom τ) (ga: groundAtom τ) (h: Option.isSome (matchAtom s a ga)): ∀ (s': substitution τ), applySubstitutionAtom s' a = ga ∧ s ⊆ s' → (Option.get (matchAtom s a ga) h) ⊆ s' :=
+by
+  unfold matchAtom at h
+  have symbol_eq: a.symbol = ga.symbol
+  by_contra p
+  simp [p] at h
+  have length_eq: a.atom_terms.length = ga.atom_terms.length
+  by_contra p
+  simp [symbol_eq, p] at h
+  simp [symbol_eq, length_eq] at h
+  unfold matchAtom
+  simp [symbol_eq, length_eq]
+  intro s'
+  unfold applySubstitutionAtom
+  unfold groundAtom.toAtom
+  simp [symbol_eq]
+  intros apply_s' s_s'
+  apply matchTermListFindsMinimalSolution (len:= length_eq)
+  constructor
+  apply apply_s'
+  apply s_s'
+
+lemma matchAtomNoneImplNoSolution (s: substitution τ) (a: atom τ) (ga: groundAtom τ) (h: Option.isNone (matchAtom s a ga)): ¬ ∃ (s': substitution τ), s ⊆ s' ∧ applySubstitutionAtom s' a = ga :=
+by
+  unfold matchAtom at h
+  by_cases symbol_eq: a.symbol = ga.symbol
+  by_cases length_eq: a.atom_terms.length = ga.atom_terms.length
+  unfold applySubstitutionAtom
+  unfold groundAtom.toAtom
+  simp [symbol_eq, length_eq] at h
+  have h': ¬∃ s', s ⊆ s' ∧ List.map (applySubstitutionTerm s') a.atom_terms = List.map term.constant ga.atom_terms
+  apply matchTermListNoneImplNoSolution (len:= length_eq) (h:= h)
+  push_neg at *
+  intros s' s_s'
+  simp [symbol_eq]
+  apply h' s' s_s'
+
+  push_neg
+  intros s' _
+  unfold groundAtom.toAtom
+  unfold applySubstitutionAtom
+  simp [symbol_eq]
+  by_contra h'
+  rw [← List.length_map a.atom_terms (applySubstitutionTerm s')] at length_eq
+  rw [← List.length_map ga.atom_terms term.constant] at length_eq
+  rw [h'] at length_eq
+  simp at length_eq
+
+  push_neg
+  intro s' _
+  unfold applySubstitutionAtom
+  unfold groundAtom.toAtom
+  simp [symbol_eq]
+
+lemma matchAtomIsSomeIffSolution (a: atom τ) (ga: groundAtom τ): Option.isSome (matchAtom emptySubstitution a ga) ↔ ∃ (s': substitution τ), applySubstitutionAtom s' a = ga :=
+by
+  constructor
+  intro h
+  use Option.get (matchAtom emptySubstitution a ga) h
+  simp [matchAtomFindsSolution]
+
+  by_contra h
+  push_neg at h
+  simp at h
+  rcases h with ⟨left,right⟩
+  have h': ¬ ∃ (s': substitution τ), emptySubstitution ⊆ s' ∧ applySubstitutionAtom s' a = ga
+  apply matchAtomNoneImplNoSolution (h:= right)
+  push_neg at h'
+  rcases left with ⟨s, s_prop⟩
+  specialize h' s (emptySubstitutionIsMinimal (τ:= τ) s)
+  exact absurd s_prop h'
+
+end atom_matching
